snap

io/IIO2.fst
@@ -18,50 +18,29 @@ match m with
 | Call cmd arg k -> forall r. contains (k r)
 | PartialCall pre k -> forall r. contains (k r)
 
-let dm_iio' = dm_iio unit trivial_hist
+type gio (flag:bool) (a:Type) = t:(dm_iio a trivial_hist){contains t ==> flag} 
+  // if the tree contains GetTrace, then the flag must be true
 
-type gio (flag:bool) = t:dm_iio'{contains t ==> flag} // if the tree contains GetTrace, then the flag must be true
-type gio_arr (flag1:bool) (flag2:bool{flag1 ==> flag2}) = 
-  #flag3:bool{flag1 ==> flag3} -> 
-    gio flag3 -> gio (flag2 || flag3) // l2 U (l3 \ l1)
-    //&& dm_iio'{(contains cin ==> contains cout) /\ ((contains cin ==> flag1) ==> (contains cout ==> flag2))}
+type gio_arr (a:Type) (flag1:bool) (b:Type) (flag2:bool{flag1 ==> flag2}) = 
+  #flag3:bool{flag1 ==> flag3} -> gio flag3 a -> gio (flag2 || flag3) b
 
-let gio_arr_apply (#flag1:bool) (#flag2:bool{flag1 ==> flag2}) (f:gio_arr flag1 flag2) (x:gio 'flag3) : Pure (gio (flag2 || 'flag3))
-  (requires (flag1 ==> 'flag3)) 
-  (ensures (fun _ -> True)) =
-  f x
-  (**
-  if flag1 = false && flag2 = false && 'flag3 = false then begin let r = f x in r end
-  else if flag1 = false && flag2 = false && 'flag3 = true then begin let r = f x in r end
-  else if flag1 = false && flag2 = true && 'flag3 = false then begin let r = f x in r end
-  else if flag1 = false && flag2 = true && 'flag3 = true then begin let r = f x in r end
-  else if flag1 = true && flag2 = true && 'flag3 = true then begin let r = f x in r end
-  else f x **)
+(** *** Proof of Concept **)
+(** we only need prog_s to use the special arrow **)
+type prog_s = gio_arr unit false unit false
+type ctx_t = m:(Type -> Type) -> m unit
 
-assume val f1 : gio_arr false false
-assume val f2 : gio_arr false true
-[@@expect_failure]
-assume val f2' : gio_arr true false
-assume val f3 : gio_arr true true
-assume val c1 : gio true
-assume val c2 : gio false
+(** ctx gets from the start instantiated with gio true **)
+let instrument (c:ctx_t) : gio true unit = c (gio true)
 
-[@@expect_failure]
-let test1' : gio false = gio_arr_apply f1 c1
-let test1 : gio true = gio_arr_apply f1 c1
-[@@expect_failure]
-let test2' : gio false = gio_arr_apply f2 c1
-let test2 : gio true = gio_arr_apply f2 c1
-[@@expect_failure]
-let test3' : gio false = gio_arr_apply f3 c1
-let test3 : gio true = gio_arr_apply f3 c1
-let test4' : gio true = gio_arr_apply f1 c2
-let test4 : gio false = gio_arr_apply f1 c2
-[@@expect_failure]
-let test5' : gio false = gio_arr_apply f2 c2
-let test5 : gio true = gio_arr_apply f2 c2
-[@@expect_failure]
-let test6 : gio true = gio_arr_apply f3 c2
+let compile_prog (p:prog_s) : (gio_arr unit true unit true) =
+  fun cs -> p cs
+
+let link (p:prog_s) (c:ctx_t) = 
+  (compile_prog p) (c (gio true))
+
+let test_type : prog_s = fun c -> 
+  io_call Openfile "../asdf"
+
 
 (** *** Lift from IO to GIO *)
 let dm_io' = dm_io unit trivial_hist
@@ -70,10 +49,44 @@ type prog_s = gio false -> gio false
 type prog_i = gio_arr false false
 
 val comp0 : prog_s -> prog_i
-let comp0 p #f c = p c
+let comp0 p #flag c = p c
 
 type prog_t = gio_arr true true 
 
 val comp1 : prog_i -> prog_t
 let comp1 p (c:gio true) =
   gio_arr_apply p c
+
+(** TESTS **)
+let gio_arr_apply (#flag1:bool) (#flag2:bool{flag1 ==> flag2}) (f:gio_arr 'a flag1 'b flag2) (x:gio 'flag3 'a) : Pure (gio (flag2 || 'flag3) 'b)
+  (requires (flag1 ==> 'flag3)) 
+  (ensures (fun _ -> True)) =
+  f x 
+
+assume val t1 : Type
+assume val t2 : Type
+
+assume val f1 : gio_arr t1 false t2 false
+assume val f2 : gio_arr t1 false t2 true
+[@@expect_failure]
+assume val f2' : gio_arr t1 true t2 false
+assume val f3 : gio_arr t1 true t2 true
+assume val c1 : gio true t1
+assume val c2 : gio false t1
+
+[@@expect_failure]
+let test1' : gio false t2 = gio_arr_apply f1 c1
+let test1 : gio true t2 = gio_arr_apply f1 c1
+[@@expect_failure]
+let test2' : gio false t2 = gio_arr_apply f2 c1
+let test2 : gio true t2 = gio_arr_apply f2 c1
+[@@expect_failure]
+let test3' : gio false t2 = gio_arr_apply f3 c1
+let test3 : gio true t2 = gio_arr_apply f3 c1
+let test4' : gio true t2 = gio_arr_apply f1 c2
+let test4 : gio false t2 = gio_arr_apply f1 c2
+[@@expect_failure]
+let test5' : gio false t2 = gio_arr_apply f2 c2
+let test5 : gio true t2 = gio_arr_apply f2 c2
+[@@expect_failure]
+let test6 : gio true t2 = gio_arr_apply f3 c2
